**2.1**  

Equation1: dES/ dt = k1*E*S – (k2+k3)ES  

Equation2: dP / dt = k3*ES

Equation3: dS / dt = k2ES - k1*E*S

Equation4: dE/ dt = (k2 + k3)ES - k1*E*S 

From Equation 1 & 4, dE/dt + dES/dt=0
Hence E(t)=E0- ES(t)  (Equation 5)
Substituting Equation 5 into equation 1 & 3:

Equation1=>  dES/ dt = k1*( E0- ES(t)  )*S – (k2+k3)ES  
	dES/ dt = k1*( E0- ES(t)  )*S – k2*ES- k3*ES
	dES/ dt = k1*( E0- ES(t)  )*S – k2*ES - dP/dt
Equation3 => dS / dt = k2ES - k1*( E0- ES(t)  )*S
Combining both, dES/dt= -dS/dt- dP/dt 
		dPdt= -dS/dt- dES/dt
